X-Wing 25519 proved correct

proof/X-Wing-Correction-Proof.ec
@@ -1,23 +1,98 @@
-require import AllCore IntDiv CoreMap List Distr.
+require import AllCore IntDiv CoreMap List Distr IntDiv StdOrder.
 
-from Jasmin require import JModel_x86.
+from Jasmin require import JModel_x86 JWord JUtils.
 
-import SLH64.
-require import XWing_Spec XWing_Helper_Functions CorrectnessProof_Mulx Mulx_scalarmult_s Jkem_avx2_stack FIPS202_SHA3 MLKEM.
+import SLH64 StdOrder.IntOrder.
+require import Jkem_avx2_clean XWing_Spec XWing_Helper_Functions CorrectnessProof_Mulx Mulx_scalarmult_s Jkem_avx2_stack FIPS202_SHA3 MLKEM Curve25519_Procedures.
 require import Array4 Array6 Array8 Array32 Array64 Array96 Array140 Array152 Array1088 Array1120 Array1184 Array1216 Array2400.
 require import WArray4 WArray6 WArray32 WArray64 WArray96 WArray1088 WArray1120 WArray1184 WArray1216 WArray2400.
-
 
 op SHA3_256_A128_A6 : W8.t Array32.t -> W8.t Array32.t -> W8.t Array32.t -> W8.t Array32.t -> W8.t Array32.t -> W8.t Array32.t.
 op SHAKE256_A96_A32 : W8.t Array96.t -> W8.t Array32.t -> W8.t Array96.t.
 
 
 axiom sha3_256_A128__A6 ss ss_mlkem ss_x25519 ct_25519 pk_25519 :
-   phoare [M._sha3_256_A128__A6 :
+   phoare [Jkem_avx2_clean.M._sha3_256_A128__A6 :
                arg = (ss, ss_mlkem, ss_x25519, ct_25519, pk_25519) ==>
                res = SHA3_256_A128_A6 ss ss_mlkem ss_x25519 ct_25519 pk_25519] = 1%r.
 
 axiom shake256_A96_A32 out inp :
-   phoare [M._shake256_A96__A32 :
+   phoare [Jkem_avx2_clean.M._shake256_A96__A32 :
                arg = (out, inp) ==>
                res = SHAKE256_A96_A32 out inp] = 1%r.
+
+abbrev toRep4 (x: W8.t Array32.t) = Array4.init (fun (i : int) => get64 (WArray32.init8 (fun (i0 : int) => x.[i0])) i).
+abbrev toRep32 (x: W64.t Array4.t) = Array32.init (fun (i : int) => get8 (WArray32.init64 (fun (i0 : int) => x.[i0])) i).
+
+lemma xwing_25519_base_mulx_equiv :
+   equiv [Jkem_avx2_clean.M.xwing_x25519_base ~ Mulx_scalarmult_s.M.__curve25519_mulx_base :
+       _k{2} = toRep4 np{1}
+       ==>
+       res{1} = toRep32 res{2}].
+    proc.
+    inline{1} 4.
+    seq 7 3 : (={u, r, k, _k}). wp. auto => />.
+    seq 4 3 : (={u, k, _k, r} /\ q{1} = r{2}). sim.
+    wp; skip => />.
+qed.
+
+lemma xwing_25519_mulx_equiv :
+   equiv [Jkem_avx2_clean.M.xwing_x25519 ~ Mulx_scalarmult_s.M.__curve25519_mulx :
+       _k{2} = toRep4 np{1}  /\
+       _u{2} = toRep4 pp{1}
+       ==>
+       res{1} = toRep32 res{2}].
+    proc.
+    inline{1} 6.
+    wp; sp.
+    sim :  (={k, u, r}).
+qed.
+
+lemma eq_spec_xwing_25519_base_mulx :
+   equiv [Jkem_avx2_clean.M.xwing_x25519_base ~ CurveProcedures.scalarmult_base :
+       Array4.of_list W64.zero (to_list (unpack64 k'{2})) = toRep4 np{1}
+       ==>
+       pack32 (to_list res{1}) = res{2}
+   ].
+    transitivity
+    Mulx_scalarmult_s.M.__curve25519_mulx_base
+    (toRep4 np{1} = _k{2} ==> res{1} = toRep32 res{2})
+    (pack4 (to_list _k{1}) = k'{2} ==> pack4 (to_list res{1}) = res{2}) => />.
+    move => &1 &2 H.
+    exists(Array4.of_list W64.zero (to_list (unpack64 k'{2}))).
+    do split.
+    + by rewrite -H. by rewrite of_listK.
+    move => &m.
+    rewrite of_listE /of_list pack32E pack4E /get8 /init64 !/to_list /(\bits8) /mkseq -iotaredE => />.
+    congr. apply fun_ext => i. rewrite !initE => />.
+    + case( 0 <= i %/ 8 && i %/ 8 < 32) => C. smt(W8.initiE). by rewrite ifF 1:/#.
+   proc *. by call xwing_25519_base_mulx_equiv.
+   proc *. symmetry. by call eq_spec_impl_scalarmult_base_mulx.
+qed.
+
+lemma eq_spec_xwing_25519_mulx :
+   equiv [Jkem_avx2_clean.M.xwing_x25519 ~ CurveProcedures.scalarmult :
+       Array4.of_list W64.zero (to_list (unpack64 k'{2})) = toRep4 np{1} /\
+       Array4.of_list W64.zero (to_list (unpack64 u'{2})) = toRep4 pp{1}
+       ==>
+       pack32 (to_list res{1}) = res{2}
+   ].
+    transitivity
+    Mulx_scalarmult_s.M.__curve25519_mulx
+    (toRep4 np{1} = _k{2} /\ toRep4 pp{1} = _u{2}
+     ==> res{1} = toRep32 res{2})
+    (pack4 (to_list _k{1}) = k'{2} /\
+     pack4 (to_list _u{1}) = u'{2}
+     ==> pack4 (to_list res{1}) = res{2}) => />.
+    move => &1 &2 H H0.
+    exists(Array4.of_list W64.zero (to_list (unpack64 k'{2})), Array4.of_list W64.zero (to_list (unpack64 u'{2}))).
+    do split.
+    + by rewrite -H. by rewrite -H0. by rewrite //= of_listK. by rewrite //= of_listK.
+    move => &m.
+    rewrite of_listE /of_list pack32E pack4E /get8 /init64 /to_list /(\bits8) /mkseq -iotaredE => />.
+    congr. apply fun_ext => i. rewrite !initE => />.
+    + case( 0 <= i %/ 8 && i %/ 8 < 32) => C. smt(W8.initiE). by rewrite ifF 1:/#.
+
+   proc *. by call xwing_25519_mulx_equiv.
+   proc *. symmetry. by call eq_spec_impl_scalarmult_mulx.
+qed.
